verif/verif_movetofirst.v
@@ -44,9 +44,99 @@ Proof.
      SEP (relation_rep r pr; cursor_rep c r pc))).
       * forward. entailer!.
       * assert_PROP(False). entailer.
-        (* contradiction in H2. *) admit.
+        admit.                  (* contradiction in H2 *)
         inv H5.
       * unfold cursor_rep.
         Intros anc_end. Intros idx_end.
         destruct r as [[[root numRec] depth] prel].
+        pose (r:=(root,numRec,depth,prel)). fold r.
+        forward.                (* cursor->ancestors[level]=node *)
+        { entailer!. unfold partial_cursor_wf in H0. destruct H0.
+          split. omega. rewrite MTD_eq in H1. auto. }
+        forward.                (* cursor->level = level *)
+        assert (partial_cursor_correct c n root) by auto.
+        apply cursor_subnode in H. unfold get_root in H. simpl in H.
+        unfold relation_rep. unfold r. Intros proot. subst pr.
+        apply subnode_rep with (proot:=proot) in H. rewrite H.
+        Intros pn0. rewrite btnode_rep_getval at 1. Intros. subst pn0. rewrite <- H1.
+        destruct n as [ptr0 le isLeaf First Last xn].
+        pose (n:=btnode val ptr0 le isLeaf First Last xn). simpl in H1. subst xn.
+        rewrite unfold_btnode_rep at 1. Intros.
+        forward.                (* t'2=node->isLeaf *)
+        { entailer!. destruct isLeaf; simpl; auto. }
+
+forward_if
+    (PROP (isLeaf=false)
+     LOCAL (temp _t'2 (Val.of_bool isLeaf); temp _cursor pc; temp _node pn;
+     temp _level (Vint (Int.repr (Zlength c))))
+     SEP (field_at Tsh trelation [StructField _root] proot prel; malloc_token Tsh tbtnode pn;
+     field_at Tsh tbtnode [StructField _numKeys]
+       (Vint (Int.repr (Z.of_nat (numKeys (btnode val ptr0 le isLeaf First Last pn))))) pn;
+     field_at Tsh tbtnode [StructField _isLeaf] (Val.of_bool isLeaf) pn;
+     field_at Tsh tbtnode [StructField _FirstLeaf] (Val.of_bool First) pn;
+     field_at Tsh tbtnode [StructField _LastLeaf] (Val.of_bool Last) pn;
+     match ptr0 with
+     | Some (@btnode _ _ _ _ _ _ p' as n') =>
+         field_at Tsh tbtnode [StructField _ptr0] p' pn * btnode_rep n' p'
+     | None => field_at Tsh tbtnode [StructField _ptr0] nullval pn
+     end; field_at Tsh tbtnode [StructField _entries] (le_to_list_complete le) pn; 
+     le_iter_sepcon le;
+     btnode_rep (btnode val ptr0 le isLeaf First Last pn) pn -* btnode_rep root proot;
+     field_at Tsh trelation [StructField _numRecords] (Vint (Int.repr (Z.of_nat numRec))) prel;
+     field_at Tsh trelation [StructField _depth] (Vint (Int.repr (Z.of_nat depth))) prel;
+     malloc_token Tsh trelation prel; malloc_token Tsh tcursor pc;
+     field_at Tsh tcursor [StructField _relation] prel pc;
+     field_at Tsh tcursor [StructField _level] (Vint (Int.repr (Zlength c))) pc;
+     field_at Tsh tcursor [StructField _ancestorsIdx]
+       (rev (map (fun x : node val * index => rep_index (snd x)) c) ++ idx_end) pc;
+     field_at Tsh tcursor [StructField _ancestors]
+       (upd_Znth (Zlength c) (rev (map getval (map fst c)) ++ anc_end)
+                 (force_val (sem_cast_pointer pn))) pc))%assert.
+{
+  - forward.                    (* cursor->ancestorsIdx[level]=0 *)
+    + entailer!. split. omega. unfold partial_cursor_wf in H0. rewrite MTD_eq in H0. destruct H0. auto.
+    + forward.                  (* return *)
+      Exists proot. normalize. cancel.
+      eapply derives_trans.
+      rewrite wand_sepcon_adjoint. rewrite wand_sepcon_adjoint. rewrite wand_sepcon_adjoint.
+      rewrite wand_sepcon_adjoint. rewrite wand_sepcon_adjoint.
+      eapply derives_trans.
+      apply wand_frame_elim.
+      rewrite <- wand_sepcon_adjoint. rewrite <- wand_sepcon_adjoint. rewrite <- wand_sepcon_adjoint.
+      rewrite <- wand_sepcon_adjoint. rewrite <- wand_sepcon_adjoint. apply derives_refl.
+      cancel.
+      unfold cursor_rep. fold n.
+      assert (Zlength ((n,ip 0)::c) -1 = Zlength c). rewrite Zlength_cons. omega.
+      rewrite H1. autorewrite with sublist. simpl.
+      Exists (sublist 1 (Zlength anc_end) anc_end). Exists (sublist 1 (Zlength idx_end) idx_end).
+      cancel. rewrite <- app_assoc. rewrite <- app_assoc.
+      rewrite upd_Znth0. rewrite upd_Znth0. cancel.
+} {
+  forward.                      (* skip *)
+  entailer!.
+  apply derives_refl.
+} {
+  forward.                      (* cursor->ancestorsidx[level]=-1 *)
+  - entailer!. split. omega. unfold partial_cursor_wf in H0. destruct H0. rewrite MTD_eq in H32. auto.
+  -                             (* recursive call *)
+    destruct ptr0 as [ptr0n|] eqn:EQPTR0.
+    + destruct ptr0n eqn:EPTR0n. Intros.
+      forward.                    (* t'1=node->ptr0 *)
+      forward_call(r,prel,((n,im)::c),pc,ptr0n,v). (* moveToFirst *)
+      * admit.                                     (* Int.min_signed <= ... <= Int.max_signed *)
+      * entailer!. repeat apply f_equal. rewrite Zlength_cons. omega.
+      * admit.                  (* relation_rep * cursor_rep *)
+      * split.
+{ admit.
+} {
+  split.
+  - admit.
+    (* we need to be able to prove that the cursor is still partial if we did the recursive call *)
+  - rewrite EPTR0n. simpl. auto.
+}
+      * forward.                (* return *)
+        Exists (getval root). entailer!.
+        admit.                  (* same cursor_rep *)
+    + admit.
+      (* ptr0 should not be None when isLeaf is false *)
 Admitted.
